Makefile
@@ -2,17 +2,24 @@
 
 COQC= coqc -Q . Elo
 
-main:
-	$(COQC) Util.v
-	$(COQC) Array.v
-	$(COQC) Map.v
-	$(COQC) Core.v
+main: core
 	$(COQC) Access.v
 	$(COQC) Compat.v
 	$(COQC) WBA.v
 	$(COQC) AccessProp.v
 	$(COQC) NoLoc.v
 	$(COQC) Disjoint.v
+
+core:
+	$(COQC) Util.v
+	$(COQC) Array.v
+	$(COQC) Map.v
+	$(COQC) Core.v
+
+soundness: core
+	$(COQC) Access.v
+	$(COQC) WBA.v
+	$(COQC) Soundness.v
 
 clean:
 	rm -f .lia.cache .*.aux *.vo *.vok *.vos *.glob
